src/core/DY.Core.Trace.SplitUtils.Derived.fst
@@ -1,0 +1,43 @@
+module DY.Core.Trace.SplitUtils.Derived
+
+open DY.Core.Trace.Type
+open DY.Core.Trace.Base
+open DY.Core.Trace.SplitUtils
+
+/// This module contains derived functions and lemmas based on
+/// trace_split, trace_concat, trace_subtract, and their properties.
+
+/// Derived functions for trace split
+
+let trace_split_grows (#label_t:Type) (tr:trace_ label_t) (ts:timestamp {ts < length tr})
+  : Lemma
+    (ensures (
+      let (tr1, e, _) = trace_split tr ts in
+      tr1 <$ tr /\
+      (Snoc tr1 e) <$ tr
+    ))
+  = trace_split_matches_prefix tr ts
+
+
+let trace_split_at (#a:Type) (tr:trace_ a) (e:trace_entry_ a{entry_exists tr e})
+  : (trace_ a & (e':trace_entry_ a{trace_entry_equiv e e'}) & trace_ a)
+  = let idx = trace_find tr e in
+    let (tr1, e', tr2) = trace_split tr idx in
+    trace_split_get_entry tr idx idx;
+    (tr1, e', tr2)
+
+/// Derived functions for trace arithmetic
+
+let trace_subtract_concat_left (#label_t:Type) (tr1 tr2 tr3:trace_ label_t)
+  : Lemma
+    (requires tr1 <$ tr2)
+    (ensures ((tr2 <--> tr1) <++> tr3) == ((tr2 <++> tr3) <--> tr1))
+  = trace_concat_assoc tr1 (tr2 <--> tr1) tr3
+
+let trace_subtract_concat_slices (#label_t:Type) (tr1 tr2 tr3:trace_ label_t)
+  : Lemma
+    (requires tr1 <$ tr2 /\ tr2 <$ tr3)
+    (ensures (tr3 <--> tr1) == ((tr2 <--> tr1) <++> (tr3 <--> tr2)))
+    [SMTPat ((tr2 <--> tr1) <++> (tr3 <--> tr2))]
+  = trace_subtract_concat_left tr1 tr2 (tr3 <--> tr2);
+    trace_subtract_concat tr3 tr2
